[Civl] UnpackCmd (#647)
* first check in

* second commit

* third commit

* eliminated NoninterferenceInstrumentation

* eliminated GlobalSnapshotInstrumentation
further simplified the interaction between permissions and noninterference checker

* more cleanup

* generalized linearTypes

* fixed typing for primitive calls

* fixed unpack typing

* added pack typing

* small fix

* pack/unpack tests

* removed local variable from desugaring
improved error message

* fixed modifies checking
handled UnpackCmd in HoistAsserts

* fixed modifies checking for pack

* added linear typing tests for pack/unpack

* amended error messages in CivlTypeChecker.cs

Source/Concurrency/CivlUtil.cs
@@ -47,7 +47,6 @@ namespace Microsoft.Boogie
       {
         errorCount += ResolveAndTypecheck(options, absy);
       }
-
       return errorCount;
     }
   }
