Source/Concurrency/NoninterferenceChecker.cs
@@ -1,4 +1,3 @@
-using System;
 using System.Collections.Generic;
 using System.Diagnostics;
 using System.Linq;
@@ -7,6 +6,16 @@ namespace Microsoft.Boogie
 {
   public static class NoninterferenceChecker
   {
+    public static string PermissionCollectorFormalName(LinearDomain domain)
+    {
+      return "linear_" + domain.DomainName + "_in";
+    }
+    
+    public static string PermissionCollectorLocalName(LinearDomain domain)
+    {
+      return "linear_" + domain.DomainName + "_available";
+    }
+    
     public static List<Declaration> CreateNoninterferenceCheckers(
       CivlTypeChecker civlTypeChecker,
       int layerNum,
@@ -22,7 +31,7 @@ namespace Microsoft.Boogie
       List<Variable> inputs = new List<Variable>();
       foreach (var domain in linearTypeChecker.LinearDomains)
       {
-        var inParam = linearTypeChecker.LinearDomainInFormal(domain);
+        var inParam = civlTypeChecker.Formal(PermissionCollectorFormalName(domain), domain.mapTypeBool, true);
         inputs.Add(inParam);
         domainToHoleVar[domain] = inParam;
       }
@@ -209,7 +218,12 @@ namespace Microsoft.Boogie
 
     private static LocalVariable CopyLocal(Variable v)
     {
-      return VarHelper.LocalVariable(v.Name, v.TypedIdent.Type);
+      var copy = VarHelper.LocalVariable(v.Name, v.TypedIdent.Type);
+      if (v.Attributes != null)
+      {
+        copy.Attributes = (QKeyValue)v.Attributes.Clone();
+      }
+      return copy;
     }
 
     private static Formal SnapshotGlobalFormal(CivlTypeChecker civlTypeChecker, Variable v)
